src/fstar/FStarC.Main.fst
@@ -273,8 +273,9 @@ let go_normal () : ML unit =
         print1 "Deps: %s\n" (show deps);
         print1 "Inclusion info: %s\n" (show tcr.mii);
         print1 "Checked module: %s\n" (show tcr.checked_module);
-        print1 "SMT decls: %s\n" (show <| fst tcr.smt_decls);
-        print1 "SMT fvars: %s\n" (show <| snd tcr.smt_decls)
+        let smt_decls = tcr.smt_decls () in
+        print1 "SMT decls: %s\n" (show <| fst smt_decls);
+        print1 "SMT fvars: %s\n" (show <| snd smt_decls)
     )
 
     (* --read_krml_file: read and print a krml file *)
